tests/acl2/rev_range.lisp
@@ -14,24 +14,63 @@
   (:some ((f0 acl2::any-p)))
   :xvar the-core-option-option-usize-)
 
-;; SKIPPED function core-iter-adapters-rev-impl-core-iter-traits-iterator-iterator-for-core-iter-adapters-rev-rev-core-ops-range-range-usize-next-core-ops-range-range-usize-: ACL2: call to an opaque/std function with no ACL2 mapping yet
+(fty::defprod core-ops-range-range-usize-
+  ((start acl2::any-p) (end acl2::any-p))
+  :xvar the-core-ops-range-range-usize-)
+
+(defun core-iter-adapters-rev-impl-core-iter-traits-iterator-iterator-for-core-iter-adapters-rev-rev-core-ops-range-range-usize-next-core-ops-range-range-usize- (self)
+  (b* ((s (core-ops-range-range-usize-->start self))
+       (e (core-ops-range-range-usize-->end self)))
+  (if (< s e)
+      (ok (cons (core-option-option-usize--some (- e 1)) (core-ops-range-range-usize- s (- e 1))))
+    (ok (cons (core-option-option-usize--none) self)))))
 
 (defun core-iter-traits-collect-impl-core-iter-traits-collect-intoiterator-for-core-iter-adapters-rev-rev-core-ops-range-range-usize-into-iter-core-iter-adapters-rev-rev-core-ops-range-range-usize- (self) (ok self))
 
 ;; SKIPPED trait/mixed declaration group (run with --monomorphize)
 
-(fty::defprod core-ops-range-range-usize-
-  ((start acl2::any-p) (end acl2::any-p))
-  :xvar the-core-ops-range-range-usize-)
+(defun core-iter-traits-iterator-iterator-rev-core-ops-range-range-usize- (self) (ok self))
 
-;; SKIPPED function core-iter-traits-iterator-iterator-rev-core-ops-range-range-usize-: ACL2: call to an opaque/std function with no ACL2 mapping yet
+(defun rev-range-sum-rev-loop0 (n iter a acc)
+  (declare (xargs :measure (nfix n)
+                  :hints (("Goal" :in-theory (theory 'ground-zero)))))
+  (if (zp n) (result-fail (err-out-of-fuel)) (b* ((n_1 (1- n)))
+  (b* (((ok v2_2) (core-iter-adapters-rev-impl-core-iter-traits-iterator-iterator-for-core-iter-adapters-rev-rev-core-ops-range-range-usize-next-core-ops-range-range-usize- iter)))
+  (b* ((acl2tmp3 v2_2)
+     (v4_4 (car acl2tmp3))
+     (iter_5 (cdr acl2tmp3)))
+  (b* ((acl2tmp6 v4_4))
+  (core-option-option-usize--case acl2tmp6
+    :none (ok acc)
+    :some (b* ((i_7 (core-option-option-usize--some->f0 acl2tmp6))) (b* (((ok v8_8) (array-index a i_7)))
+  (b* (((ok acc_9) (u32-wrapping-add acc v8_8)))
+  (rev-range-sum-rev-loop0 n_1 iter_5 a acc_9)))))))))))
 
-;; SKIPPED function rev-range-sum-rev: ACL2: call to a function that was itself skipped
+(defun rev-range-sum-rev (n a)
+  (b* (((ok v10_10) (core-iter-traits-iterator-iterator-rev-core-ops-range-range-usize- (make-core-ops-range-range-usize- :start 0 :end 8))))
+  (b* (((ok iter_11) (core-iter-traits-collect-impl-core-iter-traits-collect-intoiterator-for-core-iter-adapters-rev-rev-core-ops-range-range-usize-into-iter-core-iter-adapters-rev-rev-core-ops-range-range-usize- v10_10)))
+  (rev-range-sum-rev-loop0 n iter_11 a 0))))
 
-;; SKIPPED function rev-range-sum-rev: ACL2: call to a function that was itself skipped
+(defun rev-range-shift-up-loop0 (n iter buf)
+  (declare (xargs :measure (nfix n)
+                  :hints (("Goal" :in-theory (theory 'ground-zero)))))
+  (if (zp n) (result-fail (err-out-of-fuel)) (b* ((n_12 (1- n)))
+  (b* (((ok v13_13) (core-iter-adapters-rev-impl-core-iter-traits-iterator-iterator-for-core-iter-adapters-rev-rev-core-ops-range-range-usize-next-core-ops-range-range-usize- iter)))
+  (b* ((acl2tmp14 v13_13)
+     (v15_15 (car acl2tmp14))
+     (iter_16 (cdr acl2tmp14)))
+  (b* ((acl2tmp17 v15_15))
+  (core-option-option-usize--case acl2tmp17
+    :none (ok buf)
+    :some (b* ((i_18 (core-option-option-usize--some->f0 acl2tmp17))) (b* (((ok v19_19) (array-index buf i_18)))
+  (b* (((ok v20_20) (usize-add i_18 8)))
+  (b* (((ok v21_21) (array-update buf v20_20 v19_19)))
+  (rev-range-shift-up-loop0 n_12 iter_16 v21_21))))))))))))
 
-;; SKIPPED function rev-range-shift-up: ACL2: call to a function that was itself skipped
-
-;; SKIPPED function rev-range-shift-up: ACL2: call to a function that was itself skipped
+(defun rev-range-shift-up (n buf start)
+  (b* (((ok v22_22) (usize-add start 8)))
+  (b* (((ok v23_23) (core-iter-traits-iterator-iterator-rev-core-ops-range-range-usize- (make-core-ops-range-range-usize- :start start :end v22_22))))
+  (b* (((ok iter_24) (core-iter-traits-collect-impl-core-iter-traits-collect-intoiterator-for-core-iter-adapters-rev-rev-core-ops-range-range-usize-into-iter-core-iter-adapters-rev-rev-core-ops-range-range-usize- v23_23)))
+  (rev-range-shift-up-loop0 n iter_24 buf)))))
 
 ;; END OF GENERATED FILE
